Progress towards the verification of the add function

CoqOfPython/proofs/CoqOfPython.v
@@ -1,130 +1,214 @@
 Require Import CoqOfPython.CoqOfPython.
 
-Module State.
-  Class Trait (State Address : Set) : Type := {
+Module Stack.
+  Definition t : Set :=
+    list {A : Set @ A}.
+
+  Definition read : t -> nat -> option {A : Set @ A} :=
+    List.nth_error (A := {A : Set @ A}).
+
+  Fixpoint write {A : Set} (stack : t) (index : nat) (value : A) : t :=
+    match stack, index with
+    | start :: stack, Datatypes.O => (existS A value) :: stack
+    | start :: stack, Datatypes.S index => start :: write stack index value
+    | [], _ => []
+    end.
+
+  Lemma read_length_eq {A : Set} (stack_start stack_end : t) :
+    read (stack_start ++ stack_end) (List.length stack_start) =
+    read stack_end 0.
+  Proof.
+    now induction stack_start.
+  Qed.
+End Stack.
+
+(** The precise type of the heap is provided by the user. We only enforce some consistency
+    properties between the read and write operations. *)
+Module Heap.
+  Class Trait (Heap Address : Set) : Type := {
     get_Set (a : Address) : Set;
-    read (a : Address) : State -> option (get_Set a);
-    alloc_write (a : Address) : State -> get_Set a -> option State;
+    read (a : Address) : Heap -> option (get_Set a);
+    alloc_write (a : Address) : Heap -> get_Set a -> option Heap;
   }.
 
   Module Valid.
-    (** A valid state should behave as map from address to optional values
+    (** A valid heap should behave as map from address to optional values
         of the type given by the address. A value is [None] while not
         allocated, and [Some] once allocated. It is impossible to free
         allocated values. *)
     Record t `(Trait) : Prop := {
       (* [alloc_write] can only fail on new cells *)
-      not_allocated (a : Address) (s : State) (v : get_Set a) :
-        match alloc_write a s v with
+      not_allocated (a : Address) (h : Heap) (v : get_Set a) :
+        match alloc_write a h v with
         | Some _ => True
-        | None => read a s = None
+        | None => read a h = None
         end;
-      same (a : Address) (s : State) (v : get_Set a) :
-        match alloc_write a s v with
-        | Some s => read a s = Some v
+      same (a : Address) (h : Heap) (v : get_Set a) :
+        match alloc_write a h v with
+        | Some h => read a h = Some v
         | None => True
         end;
-      different (a1 a2 : Address) (s : State) (v2 : get_Set a2) :
+      different (a1 a2 : Address) (h : Heap) (v2 : get_Set a2) :
         a1 <> a2 ->
-        match alloc_write a2 s v2 with
-        | Some s' => read a1 s' = read a1 s
+        match alloc_write a2 h v2 with
+        | Some h' => read a1 h' = read a1 h
         | None => True
         end;
         }.
   End Valid.
-End State.
+End Heap.
 
 Module Run.
-  Reserved Notation "{{ state | e ⇓ result | state' }}".
+  Reserved Notation "{{ stack , heap | e ⇓ result | stack' , heap' }}".
 
-  Inductive t `{State.Trait} {A : Set}
-      (* Be aware of the order of parameters: the result and final state are at
+  Inductive t `{Heap.Trait} {A : Set}
+      (* Be aware of the order of parameters: the result and final heap are at
          the beginning. This is due to the way polymorphic types for inductive
          work in Coq, and the fact that the result is always the same as we are
          in continuation passing style. *)
-      (result : A) (state' : State) :
-      LowM.t A -> State -> Prop :=
+      {result : A} {stack' : Stack.t} {heap' : Heap} :
+      LowM.t A -> Stack.t -> Heap -> Prop :=
   | Pure :
-    {{ state' | LowM.Pure result ⇓ result | state' }}
+    {{ stack', heap' |
+      LowM.Pure result ⇓
+      result
+    | stack', heap' }}
   | CallPrimitiveStateAllocImmediate
-      (state : State) (object : Object.t Value.t)
+      (stack : Stack.t) (heap : Heap) (object : Object.t Value.t)
       (k : Pointer.t Value.t -> LowM.t A) :
-    {{ state |
-      k (Pointer.Imm object) ⇓ result
-    | state' }} ->
-    {{ state |
-      LowM.CallPrimitive (Primitive.StateAlloc object) k ⇓ result
-    | state' }}
-  | CallPrimitiveStateAllocMutable
-      (address : Address)
-      (value : State.get_Set address)
+    {{ stack, heap |
+      k (Pointer.Imm object) ⇓
+      result
+    | stack', heap' }} ->
+    {{ stack, heap |
+      LowM.CallPrimitive (Primitive.StateAlloc object) k ⇓
+      result
+    | stack', heap' }}
+  | CallPrimitiveStateAllocStack {B : Set}
+      (value : B)
+      (to_object : B -> Object.t Value.t)
       (object : Object.t Value.t)
-      (to_object : State.get_Set address -> Object.t Value.t)
-      (state : State)
+      (stack : Stack.t) (heap : Heap)
       (k : Pointer.t Value.t -> LowM.t A) :
+    let stack_inter := (stack ++ [existS B value])%list in
+    let index := List.length stack in
+    let mutable := Pointer.Mutable.Stack index to_object in
     object = to_object value ->
-    State.read address state = None ->
-    State.alloc_write address state value = Some state' ->
-    {{ state |
-      k (Pointer.Mutable (Pointer.Mutable.Make address to_object)) ⇓ result
-    | state' }} ->
-    {{ state |
-      LowM.CallPrimitive (Primitive.StateAlloc object) k ⇓ result
-    | state' }}
-  | CallPrimitiveStateRead
+    {{ stack_inter, heap |
+      k (Pointer.Mutable mutable) ⇓
+      result
+    | stack', heap' }} ->
+    {{ stack, heap |
+      LowM.CallPrimitive (Primitive.StateAlloc object) k ⇓
+      result
+    | stack', heap' }}
+  | CallPrimitiveStateAllocHeap
       (address : Address)
-      (to_object : State.get_Set address -> Object.t Value.t)
-      (value : State.get_Set address)
-      (state : State)
+      (value : Heap.get_Set address)
+      (object : Object.t Value.t)
+      (to_object : Heap.get_Set address -> Object.t Value.t)
+      (stack : Stack.t) (heap heap_inter : Heap)
+      (k : Pointer.t Value.t -> LowM.t A) :
+    let mutable := Pointer.Mutable.Heap address to_object in
+    object = to_object value ->
+    Heap.read address heap = None ->
+    Heap.alloc_write address heap value = Some heap_inter ->
+    {{ stack, heap_inter |
+      k (Pointer.Mutable mutable) ⇓
+      result
+    | stack', heap' }} ->
+    {{ stack, heap |
+      LowM.CallPrimitive (Primitive.StateAlloc object) k ⇓
+      result
+    | stack', heap' }}
+  | CallPrimitiveStateReadStack {B : Set}
+      (index : nat)
+      (to_object : B -> Object.t Value.t)
+      (value : B)
+      (stack : Stack.t) (heap : Heap)
       (k : Object.t Value.t -> LowM.t A) :
-    let mutable := Pointer.Mutable.Make address to_object in
-    State.read address state = Some value ->
-    {{ state |
+    let mutable := Pointer.Mutable.Stack index to_object in
+    Stack.read stack index = Some (existS B value) ->
+    {{ stack, heap |
       k (to_object value) ⇓
       result
-    | state' }} ->
-    {{ state |
+    | stack', heap' }} ->
+    {{ stack, heap |
       LowM.CallPrimitive (Primitive.StateRead mutable) k ⇓
       result
-    | state' }}
-  | CallPrimitiveStateWrite
+    | stack', heap' }}
+  | CallPrimitiveStateReadHeap
       (address : Address)
-      (to_object : State.get_Set address -> Object.t Value.t)
-      (update : State.get_Set address)
+      (to_object : Heap.get_Set address -> Object.t Value.t)
+      (value : Heap.get_Set address)
+      (stack : Stack.t) (heap : Heap)
+      (k : Object.t Value.t -> LowM.t A) :
+    let mutable := Pointer.Mutable.Heap address to_object in
+    Heap.read address heap = Some value ->
+    {{ stack, heap |
+      k (to_object value) ⇓
+      result
+    | stack', heap' }} ->
+    {{ stack, heap |
+      LowM.CallPrimitive (Primitive.StateRead mutable) k ⇓
+      result
+    | stack', heap' }}
+  | CallPrimitiveStateWriteStack {B : Set}
+      (index : nat)
+      (to_object : B -> Object.t Value.t)
+      (update : B)
       (update' : Object.t Value.t)
-      (state state_inter : State)
+      (stack : Stack.t) (heap : Heap)
       (k : unit -> LowM.t A) :
-    let mutable := Pointer.Mutable.Make address to_object in
+    let stack_inter := Stack.write stack index update in
+    let mutable := Pointer.Mutable.Stack index to_object in
     update' = to_object update ->
-    State.alloc_write address state update = Some state_inter ->
-    {{ state_inter |
+    {{ stack_inter, heap |
       k tt ⇓
       result
-    | state' }} ->
-    {{ state |
+    | stack', heap' }} ->
+    {{ stack, heap |
       LowM.CallPrimitive (Primitive.StateWrite mutable update') k ⇓
       result
-    | state' }}
+    | stack', heap' }}
+  | CallPrimitiveStateWriteHeap
+      (address : Address)
+      (to_object : Heap.get_Set address -> Object.t Value.t)
+      (update : Heap.get_Set address)
+      (update' : Object.t Value.t)
+      (stack : Stack.t) (heap heap_inter : Heap)
+      (k : unit -> LowM.t A) :
+    let mutable := Pointer.Mutable.Heap address to_object in
+    update' = to_object update ->
+    Heap.alloc_write address heap update = Some heap_inter ->
+    {{ stack, heap_inter |
+      k tt ⇓
+      result
+    | stack', heap' }} ->
+    {{ stack, heap |
+      LowM.CallPrimitive (Primitive.StateWrite mutable update') k ⇓
+      result
+    | stack', heap' }}
   | CallClosure
-      (state state_inter : State)
+      (stack stack_inter : Stack.t) (heap heap_inter : Heap)
       (f : Value.t -> Value.t -> M)
       (args kwargs : Value.t)
       (value : Value.t + Exception.t)
       (k : Value.t + Exception.t -> LowM.t A) :
     let closure := Data.Closure f in
-    {{ state |
+    {{ stack, heap |
       f args kwargs ⇓
       value
-    | state_inter }} ->
-    {{ state_inter |
+    | stack_inter, heap_inter }} ->
+    {{ stack_inter, heap_inter |
       k value ⇓
       result
-    | state' }} ->
-    {{ state |
+    | stack', heap' }} ->
+    {{ stack, heap |
       LowM.CallClosure closure args kwargs k ⇓
       result
-    | state' }}
+    | stack', heap' }}
 
-  where "{{ state | e ⇓ result | state' }}" :=
-    (t result state' e state).
+  where "{{ stack , heap | e ⇓ result | stack' , heap' }}" :=
+    (t (result := result) (stack' := stack') (heap' := heap') e stack heap).
 End Run.
